more grind

LeroyCompilerVerificationCourse/Deadcode.lean
@@ -7,29 +7,25 @@ Authors: Wojciech Różowski
 import LeroyCompilerVerificationCourse.Imp
 import Std.Data.HashSet
 
-open Classical in
-@[grind] def IdentSet := Std.HashSet ident
-  deriving Membership, Union, EmptyCollection
+abbrev IdentSet := Std.HashSet ident
 
-@[grind] instance : HasSubset IdentSet where
+instance : HasSubset IdentSet where
   Subset (a b : IdentSet) := ∀ x ∈ a, x ∈ b
 
-@[grind] noncomputable instance (a b : IdentSet) : Decidable (a ⊆ b) := Classical.propDecidable (a ⊆ b)
+noncomputable instance (a b : IdentSet) : Decidable (a ⊆ b) := Classical.propDecidable (a ⊆ b)
 
-@[grind] instance (x : ident) (a : IdentSet) : Decidable (x ∈ a) := Std.HashSet.instDecidableMem
-
-@[grind] instance : EmptyCollection IdentSet where
+instance : EmptyCollection IdentSet where
   emptyCollection := Std.HashSet.emptyWithCapacity
 
-@[grind] axiom union_characterisation (a b : IdentSet) (x : ident) : x ∈ (a ∪ b) ↔ x ∈ a ∨ x ∈ b
+@[grind =] theorem subset_def (a b : IdentSet) : a ⊆ b ↔ ∀ x ∈ a, x ∈ b := Iff.rfl
+
+@[grind] axiom union_characterisation (a b : IdentSet) (x : ident) : x ∈ a ∪ b ↔ x ∈ a ∨ x ∈ b
 
 @[grind] theorem union_characterisation2 (a b c : IdentSet) : a ⊆ b ∧ a ⊆ c → a ⊆ (b ∪ c) := by
-  intro ⟨ m1 , m2 ⟩
-  intro y mem
-  specialize m1 y mem
-  specialize m2 y mem
+  intro ⟨m1, m2⟩
+  intro y
+  specialize m1 y
   grind
-
 
 @[grind] theorem insert_characterisation (a : IdentSet) (x : ident) : x ∈ a.insert x := by
   grind
@@ -70,26 +66,16 @@ open Classical in
 
 @[grind] theorem  fixpoint_charact' (n : Nat) (x : IdentSet)  (F : IdentSet → IdentSet) (default : IdentSet) :
   ((F (deadcode_fixpoint_rec F default n x)) ⊆ (deadcode_fixpoint_rec F default n x)) ∨ (deadcode_fixpoint_rec F default n x = default) := by
-    induction n generalizing x <;> grind
+    induction n generalizing x with grind
 
 theorem fixpoint_charact (F : IdentSet → IdentSet) (default : IdentSet) :
     ((F (deadcode_fixpoint F default)) ⊆ (deadcode_fixpoint F default)) ∨ (deadcode_fixpoint F default = default) := by grind
 
+@[grind]
 theorem fixpoint_upper_bound (F : IdentSet → IdentSet) (default : IdentSet) (F_stable : ∀ x , x ⊆ default -> (F x) ⊆ default) : deadcode_fixpoint F default ⊆ default := by
   have : ∀ n : Nat, ∀ x : IdentSet, x ⊆ default → (deadcode_fixpoint_rec F default n x) ⊆ default := by
     intro n
-    induction n
-    case zero =>
-      intro x contained
-      simp [deadcode_fixpoint_rec]
-      unfold Subset
-      unfold instHasSubsetIdentSet
-      grind
-    case succ n ih =>
-      grind
-  apply this
-  unfold Subset
-  unfold instHasSubsetIdentSet
+    induction n with grind
   grind
 
 @[grind] noncomputable def live (c : com) (L : IdentSet) : IdentSet :=
@@ -108,106 +94,16 @@ theorem fixpoint_upper_bound (F : IdentSet → IdentSet) (default : IdentSet) (F
       let default := (fv_com (.WHILE b c)) ∪ L
       deadcode_fixpoint (fun x => L' ∪ (live c x)) default
 
+@[grind]
 theorem live_upper_bound :
   ∀ c L,
-   (live c L) ⊆ ((fv_com c) ∪  L) := by
+   (live c L) ⊆ ((fv_com c) ∪ L) := by
     intro c
-    induction c
-    case SKIP =>
-      intro L
-      simp [fv_com, live]
-      unfold Subset
-      unfold instHasSubsetIdentSet
-      grind
-    case ASSIGN x a =>
-      intro L
-      simp [fv_com, live]
-      split
-      case isTrue h =>
-        unfold Subset
-        unfold instHasSubsetIdentSet
-        grind
-      case isFalse h =>
-        unfold Subset
-        unfold instHasSubsetIdentSet
-        grind
-    case SEQ c1 c2 c1_ih c2_ih =>
-      intro L
-      simp [live, fv_com]
-      unfold Subset at *
-      unfold instHasSubsetIdentSet at *
-      simp at *
-      intro x contained
-      specialize c1_ih (live c2 L) x contained
-      grind
-    case IFTHENELSE b c1 c2 c1_ih c2_ih =>
-      unfold Subset at *
-      unfold instHasSubsetIdentSet at *
-      simp at *
-      grind
-    case WHILE b c1 c1_ih =>
-      simp [live, fv_com]
-      intro L
-      apply fixpoint_upper_bound
-      intro x hyp
-      intro y hyp2
-      have : y ∈ fv_bexp b ∨ y ∈ L ∨ y ∈ live c1 x := by grind
-      apply Or.elim this
-      next =>
-        grind
-      next =>
-        intro hyp3
-        apply Or.elim hyp3
-        next => grind
-        next =>
-          clear hyp3
-          intro hyp3
-          specialize c1_ih x y hyp3
-          have : y ∈ fv_com c1 ∨ y ∈ x := by grind
-          apply Or.elim this
-          next => grind
-          next =>
-            intro hyp4
-            specialize hyp y hyp4
-            grind
+    induction c with grind
 
 theorem live_while_charact (b : bexp) (c : com) (L L' : IdentSet)
   (eq : L' = live (.WHILE b c) L) :
-  (fv_bexp b) ⊆ L' ∧ L ⊆ L' ∧ (live c L') ⊆ L' := by
-    have hyp := fixpoint_charact (fun x : IdentSet => (fv_bexp b) ∪ L ∪ (live c x)) ((fv_bexp b) ∪ (fv_com c) ∪ L)
-    apply Or.elim hyp
-    case left =>
-      intro included
-      constructor
-      case left =>
-        intro y contained
-        specialize included y
-        grind
-      case right =>
-        constructor
-        case left =>
-          intro y mem
-          specialize included y
-          grind
-        case right =>
-          intro y mem
-          specialize included y
-          grind
-    case right =>
-      intro equal
-      constructor
-      case left =>
-        intro y mem
-        grind
-      case right =>
-        constructor
-        case left =>
-          intro y mem
-          grind
-        case right =>
-          intro y mem
-          have := live_upper_bound c L' y mem
-          grind
+  (fv_bexp b) ⊆ L' ∧ L ⊆ L' ∧ (live c L') ⊆ L' := by grind
 
 @[grind] noncomputable def dce (c : com) (L : IdentSet) : com :=
   match c with
@@ -222,13 +118,7 @@ theorem live_while_charact (b : bexp) (c : com) (L L' : IdentSet)
 
 @[grind] theorem agree_mon :
   ∀ L L' s1 s2,
-  agree L' s1 s2 -> L ⊆ L' -> agree L s1 s2 := by
-    intro L L' s1 s2 AG sub
-    unfold agree at *
-    intro x inL
-    specialize sub x inL
-    specialize AG x sub
-    exact AG
+  agree L' s1 s2 -> L ⊆ L' -> agree L s1 s2 := by grind
 
 @[grind] theorem aeval_agree :
   ∀ L s1 s2, agree L s1 s2 ->
@@ -238,129 +128,23 @@ theorem live_while_charact (b : bexp) (c : com) (L L' : IdentSet)
     any_goals grind
     case VAR x =>
       simp [fv_aexp]
-      intro mem
-      have : x ∈ L := by
-        have := insert_characterisation ∅ x
-        specialize mem x this
-        exact mem
-      simp [aeval]
-      unfold agree at AG
-      specialize AG x this
-      exact AG
-    case PLUS a1 a2 a1_ih a2_ih =>
-      intro contained
-      simp [aeval]
-      congr 1
-      next =>
-        apply a1_ih
-        simp [fv_aexp] at contained
-        intro y mem
-        specialize contained y (by grind)
-        exact contained
-      next =>
-        apply a2_ih
-        simp [fv_aexp] at contained
-        intro y mem
-        specialize contained y (by grind)
-        exact contained
-    case MINUS a1 a2 a1_ih a2_ih =>
-      intro contained
-      simp [aeval]
-      congr 1
-      next =>
-        apply a1_ih
-        simp [fv_aexp] at contained
-        intro y mem
-        specialize contained y (by grind)
-        exact contained
-      next =>
-        apply a2_ih
-        simp [fv_aexp] at contained
-        intro y mem
-        specialize contained y (by grind)
-        exact contained
+      grind
 
 theorem beval_agree :
   ∀ L s1 s2, agree L s1 s2 ->
   ∀ b, (fv_bexp b) ⊆ L -> beval s1 b = beval s2 b := by
     intro L s1 s2 AG b
-    induction b
-    any_goals grind
-    case EQUAL a1 a2 =>
-      intro cont
-      unfold agree at AG
-      simp [fv_bexp] at cont
-      have aeval_lemma := aeval_agree L s1 s2 AG
-      have subgoal1 : fv_aexp a1 ⊆ L := by
-        intro y mem
-        specialize cont y (by grind)
-        exact cont
-      have subgoal2 : fv_aexp a2 ⊆ L := by
-        intro y mem
-        specialize cont y (by grind)
-        exact cont
-      have eq1 := aeval_lemma a1 subgoal1
-      have eq2 := aeval_lemma a2 subgoal2
-      grind
-    case LESSEQUAL a1 a2 =>
-      intro cont
-      unfold agree at AG
-      simp [fv_bexp] at cont
-      have aeval_lemma := aeval_agree L s1 s2 AG
-      have subgoal1 : fv_aexp a1 ⊆ L := by
-        intro y mem
-        specialize cont y (by grind)
-        exact cont
-      have subgoal2 : fv_aexp a2 ⊆ L := by
-        intro y mem
-        specialize cont y (by grind)
-        exact cont
-      have eq1 := aeval_lemma a1 subgoal1
-      have eq2 := aeval_lemma a2 subgoal2
-      grind
-    case AND b1 b2 b1_ih b2_ih =>
-      intro cont
-      simp [fv_bexp] at cont
-      have : fv_bexp b1 ⊆ L ∧ fv_bexp b2 ⊆ L := by
-        constructor
-        case left =>
-          intro y mem
-          specialize cont y (by grind)
-          exact cont
-        case right =>
-          intro y mem
-          specialize cont y (by grind)
-          exact cont
-      specialize b1_ih (by grind)
-      specialize b2_ih (by grind)
-      grind
+    induction b with grind
 
 theorem agree_update_live :
   ∀ s1 s2 L x v,
   agree (L.erase x) s1 s2 ->
-  agree L (update x v s1) (update x v s2) := by
-    intro s1 s2 L x v AG
-    unfold agree at *
-    intro y
-    specialize AG y
-    intro inL
-    by_cases x = y
-    case neg notEq =>
-      specialize AG (by grind)
-      grind
-    case pos isEq =>
-      grind
+  agree L (update x v s1) (update x v s2) := by grind
 
 theorem agree_update_dead :
   ∀ s1 s2 L x v,
   agree L s1 s2 -> ¬x ∈ L ->
-  agree L (update x v s1) s2 := by
-    intro s1 s2 L x v AG not
-    unfold agree at *
-    intro y mem
-    specialize AG y mem
-    simp [update]
-    by_cases x=y <;> grind
+  agree L (update x v s1) s2 := by grind
 
 theorem dce_correct_terminating :
   ∀ s c s', cexec s c s' ->
@@ -371,19 +155,14 @@ theorem dce_correct_terminating :
     any_goals grind
     case cexec_while_loop s1 b c1 s2 s3 isTrue EX1 EX2 a_ih a_ih2 =>
       intro L s4 hyp
-      have := live_while_charact b c1 L  (live (com.WHILE b c1) L) (by grind)
-      have : agree (live c1 (live (com.WHILE b c1) L)) s1 s4 := by
-        apply agree_mon
-        · exact hyp
-        · grind
-      have ⟨ t1, ht1, ht2⟩ :=  a_ih (live (.WHILE b c1) L) s4 this
-      have ⟨u1, hu1, hu2 ⟩ :=  a_ih2 L t1 ht2
+      have ⟨t1, ht1, ht2⟩ :=  a_ih (live (.WHILE b c1) L) s4 (by grind)
+      have ⟨u1, hu1, hu2⟩ :=  a_ih2 L t1 ht2
       exists u1
       constructor
       rotate_right
       · exact hu2
       · apply cexec.cexec_while_loop
-        · have := beval_agree (live (com.WHILE b c1) L) s1 s4 hyp b (by grind)
+        · have := beval_agree (live (com.WHILE b c1) L) s1 s4
           grind
         · exact ht1
         · grind
@@ -393,64 +172,31 @@ theorem dce_correct_terminating :
       by_cases x ∈ L
       case neg notIn =>
         exists s3
-        constructor
-        · grind [dce]
-        · simp [notIn] at AG
-          exact @agree_update_dead s2 s3 L x (aeval s2 a) (by grind) notIn
+        grind
       case pos isIn =>
-        simp [isIn] at AG
         exists (update x (aeval s3 a) s3)
-        constructor
-        · simp [dce, isIn]
-          grind
-        · have subgoal : aeval s2 a = aeval s3 a := by
-            apply aeval_agree
-            · exact AG
-            · intro y mem
-              grind
-          rw [subgoal]
-          apply @agree_update_live
-          grind
+        grind
     case cexec_ifthenelse s2 b c1 c2 s3 EXEC ih =>
       intro L s4 AG
       simp [dce]
       have EQ : beval s2 b = beval s4 b := by
         apply beval_agree
         · apply AG
-        · simp [live]
-          intro y mem
-          grind
+        · grind
       by_cases beval s2 b = true
       case pos isTrue =>
-        simp [isTrue] at EXEC
         specialize ih L s4
-        simp [live] at AG
-        simp [isTrue] at ih
-        have ⟨s5 , EX', AG' ⟩ := ih (by grind)
-        exists s5
-        constructor
-        · apply cexec.cexec_ifthenelse
-          grind
-        · exact AG'
+        grind
       case neg isFalse =>
-        simp [isFalse] at EXEC
         specialize ih L s4
-        simp [live] at AG
-        simp [isFalse] at ih
-        have ⟨s5 , EX', AG' ⟩ := ih (by grind)
-        exists s5
-        constructor
-        · apply cexec.cexec_ifthenelse
-          grind
-        · exact AG'
+        grind
     case cexec_while_done s2 b c isFalse =>
       intro L s1 AG
-      have ⟨ h1 , h2 , h3 ⟩ := live_while_charact b c L (live (com.WHILE b c) L) (by grind)
+      have ⟨h1, h2, h3⟩ := live_while_charact b c L (live (com.WHILE b c) L) (by grind)
       have EQ : beval s2 b = beval s1 b := by
         apply beval_agree
         · apply AG
-        · intro y mem
-          specialize h1 y mem
-          exact h1
+        · grind
       exists s1
       grind
+    case cexec_seq => grind [-subset_def] -- TODO: what does wrong?
